Update HW7 Bonus_1.dfy

HW7 Bonus_1.dfy
@@ -1,34 +1,28 @@
-predicate Sorted(A: array<int>, lo: int, hi: int)
-    reads A
-    requires 0 <= lo <= hi <= A.Length
-{
-    forall i, j :: lo <= i <= j < hi ==> A[i] <= A[j]
-}
-
-
 method InsertionSort(n: int, A: array<int>)
   requires n == A.Length
   modifies A
-  ensures  Sorted(A, 0, n)              
+  ensures Sorted(A, 0, n)              
 {
-  if n <= 1 { return; } // Length 1 is automatically sorted
+  if n <= 1 { return; }
 
   var i := 1;
   while i < n
     invariant 1 <= i <= n
-    //invariant Sorted(___________________) // Please fill in
-    //decreases ___________________________ // Please fill in
+    invariant Sorted(A, 0, i)
+    decreases n - i
   {
     var j := i;
-    // Shift elements greater than Ai one position to the right
+    // Shift elements greater than A[i] one position to the right
     while j >= 1 && A[j-1] > A[j]
       invariant 0 <= j <= i
-      //invariant Sorted(___________________) // Please fill in
-      //decreases ___________________________ // Please fill in
+      invariant Sorted(A, 0, i)
+      invariant forall k :: j <= k <= i ==> A[k] >= A[j]
+      invariant forall k, l :: 0 <= k < j && j <= l <= i ==> A[k] <= A[l]
+      decreases j
     {
-      A[j-1],A[j] := A[j], A[j-1]; // swap A[j-1] with A[j]
+      A[j-1], A[j] := A[j], A[j-1];
       j := j - 1;
-    } // end while j >= 1 && A[j-1] > A[j]
+    }
     i := i + 1;
-  } // end while i < n
+  }
 }
